# 回归算法

Define the following quantities:
$$
y
= \left[ \begin{array}
{c} y_1 \\ \vdots \\ y_n
\end{array}\right]
=\left[y_{1}, \cdots, y_{n}\right]^{T}     \quad (n×1)
$$

$$
\phi(x)= [1,x,,x^2,\cdots,x^K]^T   \quad (k+1×1)
$$

$$
\Phi = \left[\phi(x_1), \cdots, \phi(x_n)\right] \quad (1×n)
$$

$$
X=\left[x_1, \cdots,x_n\right] \quad (1×n)
$$

$$
\theta = [\theta_0, \cdots ,\theta_K]^T \quad (K×1)
$$



## 1、least-squares (LS)

objective function $\left\|y-\Phi^{T} \theta\right\|^{2}$
$$
\begin{aligned}
\underset{\theta}{argmin} \left\|y-\Phi^{T} \theta\right\|^{2}
&= \underset{\theta}{argmin} (y-\Phi^T\theta)^T(y-\Phi^T\theta) \\
&= \underset{\theta}{argmin} (y^T-\theta^T\Phi)(y-\Phi^T\theta) \\
&= \underset{\theta}{argmin} [y^Ty-y^T\Phi^T\theta-\theta^T\Phi y+\theta^T\Phi\Phi^T\theta] \\
(y^T\Phi^T\theta是实数，所以类似A^T=A)&= \underset{\theta}{argmin} [y^Ty-2y^T\Phi^T\theta+\theta^T\Phi\Phi^T\theta]
\end{aligned}
$$
derivatives
$$
\begin{aligned}
\frac{\partial}{\partial\theta}[y^Ty-2y^T\Phi^T\theta+\theta^T\Phi\Phi^T\theta]
& = 2\Phi y + \Phi\Phi^T\theta + \theta^T\Phi\Phi^T \\
(还是因为实数)& = -2\Phi y +2\Phi \Phi^T \theta
\end{aligned}
$$
because $\frac{\partial x^T a}{\partial{x}}=\frac{\partial a^T x}{\partial{x}} = a $  and $\partial x^T= (\partial x)^T$ 

$$
-2\Phi y +2\Phi \Phi^T \theta = 0 \Longrightarrow \theta = (\Phi\Phi^T)^{-1}\Phi y
$$
parameter estimate:
$$
\hat{\theta} = (\Phi\Phi^T)^{-1}\Phi y
$$


## 2、regularized LS (RLS)

objective function $\left\|y-\Phi^{T} \theta\right\|^{2} + \lambda \|\theta\|^2$
$$
\begin{aligned}
\underset{\theta}{argmin} \left\|y-\Phi^{T} \theta\right\|^{2} + \lambda \|\theta\|^2
&= \underset{\theta}{argmin} (y-\Phi^T\theta)^T(y-\Phi^T\theta) + \lambda \theta^T \theta \\
&= \underset{\theta}{argmin} (y^T-\theta^T\Phi)(y-\Phi^T\theta) + \lambda \theta^T \theta\\
&= \underset{\theta}{argmin} [y^Ty-y^T\Phi^T\theta-\theta^T\Phi y+\theta^T\Phi\Phi^T\theta + \lambda \theta^T \theta ] \\
(y^T\Phi^T\theta是实数，所以类似A^T=A)&= \underset{\theta}{argmin} [y^Ty-2y^T\Phi^T\theta+\theta^T\Phi\Phi^T\theta + \lambda \theta^T \theta]
\end{aligned}
$$
derivatives
$$
\begin{aligned}
\frac{\partial}{\partial\theta}[y^Ty-2y^T\Phi^T\theta+\theta^T\Phi\Phi^T\theta+ \lambda \theta^T \theta]
& = 2\Phi y + \Phi\Phi^T\theta + \theta^T\Phi\Phi^T + 2 \lambda \theta \\
(还是因为实数)& = -2\Phi y +2\Phi \Phi^T \theta + 2 \lambda \theta
\end{aligned}
$$
because $\frac{\partial x^Tx}{\partial{x}} = 2x$
$$
-2\Phi y +2\Phi \Phi^T \theta + 2 \lambda \theta = 0 \Longrightarrow \theta =(\Phi\Phi^T+\lambda I)^{-1}\Phi y
$$
parameter estimate:
$$
\hat{\theta} = (\Phi\Phi^T+\lambda I)^{-1}\Phi y
$$

## 3、L1-regularized LS (LASSO)

objective function $\left\|y-\Phi^{T} \theta\right\|^{2} + \lambda \|\theta\|_1$